src/lib/communication/DY.Lib.Communication.RequestResponse.Lemmas.fst
@@ -2,8 +2,7 @@ module DY.Lib.Communication.RequestResponse.Lemmas
 
 open Comparse
 open DY.Core
-open DY.Lib.Communication.Core.Extension
-open DY.Lib.Crypto.PkEncryption.Split
+open DY.Lib.Crypto.PKE.Split
 open DY.Lib.Crypto.Signature.Split
 open DY.Lib.State.PKI
 open DY.Lib.State.PrivateKeys
